Encode string length and concat operator
Co-authored-by: A L Manning <asher@zenprotocol.com>

src/smtencoding/FStarC.SMTEncoding.Util.fst
@@ -83,6 +83,8 @@ let mkBvUlt = norng mkBvUlt
 let mkBvUext sz = norng (mkBvUext sz)
 let mkBvToNat = norng mkBvToNat
 let mkITE = norng mkITE
+let mkStrLen = norng mkStrLen
+let mkStrCat = norng mkStrCat
 let mkCases = norng mkCases
 
 let norng2 f = fun x y -> f x y Range.dummyRange
