src/smtencoding/FStarC.SMTEncoding.Util.fsti
@@ -59,6 +59,8 @@ val mkDiv : term & term -> term
 val mkRealDiv : term & term -> term
 val mkMul : term & term -> term
 val mkMod : term & term -> term
+val mkStrLen : term -> term
+val mkStrCat : term & term -> term
 
 (* bitvector ops, some indexed by bitvector size *)
 val mkNatToBv : int -> term -> term
